Some changes in the transformation and progress proving its functionality.

Transformation.v
@@ -24,48 +24,48 @@ Definition C' : typdefctx := (\{})["pos" := pos'].
 
 (* Grouping transformation *)
 Record group_tr := make_group_tr {
-  group_tr_struct_name : typvar;
-  group_tr_new_struct_name : typvar;
-  group_tr_fields : list field
+  group_tr_struct_name : typvar; (* s *)
+  group_tr_fields : list field; (* [..f..] *)
+  group_tr_new_struct_name : typvar; (* s_g *)
+  group_tr_new_struct_field : field (* f_g *)
 }.
 
 (* π ~ |π| *)
-Inductive tr_accesses : group_tr -> accesses -> accesses -> Prop :=
-  | tr_accesses_nil : forall gt,
+Inductive tr_accesses (gt:group_tr) : accesses -> accesses -> Prop :=
+  | tr_accesses_nil : 
       tr_accesses gt nil nil
-  | tr_accesses_array : forall gt π π' i,
+  | tr_accesses_array : forall π π' i,
       tr_accesses gt π π' ->
       tr_accesses gt ((access_array i)::π) ((access_array i)::π')
-  | tr_accesses_field_group : forall gt π π' f f',
+  | tr_accesses_field_group : forall π π' f f_g,
       tr_accesses gt π π' ->
-      List.In f (group_tr_fields gt) ->
-      f' = group_tr_new_struct_name gt ->
-      tr_accesses gt ((access_field f)::π) ((access_field f')::(access_field f)::π')
-  | tr_accesses_field_other : forall gt π π' f,
+      mem f (group_tr_fields gt) ->
+      f_g = group_tr_new_struct_field gt ->
+      tr_accesses gt ((access_field f)::π) ((access_field f_g)::(access_field f)::π')
+  | tr_accesses_field_other : forall π π' f,
       tr_accesses gt π π' ->
-      ~ List.In f (group_tr_fields gt) ->
+      ~ mem f (group_tr_fields gt) ->
       tr_accesses gt ((access_field f)::π) ((access_field f)::π').
 
 (* v ~ |v| *)
-Inductive tr_val : group_tr -> val -> val -> Prop :=
-  | tr_val_unit : forall gt,
+Inductive tr_val (gt:group_tr) : val -> val -> Prop :=
+  | tr_val_unit : 
       tr_val gt val_unit val_unit
-  | tr_val_bool : forall gt b,
+  | tr_val_bool : forall b,
       tr_val gt (val_bool b) (val_bool b)
-  | tr_val_int : forall gt i,
+  | tr_val_int : forall i,
       tr_val gt (val_int i) (val_int i)
-  | tr_val_double : forall gt d,
+  | tr_val_double : forall d,
       tr_val gt (val_double d) (val_double d)
-  | tr_val_abstract_ptr : forall gt l π π',
+  | tr_val_abstract_ptr : forall l π π',
       tr_accesses gt π π' ->
       tr_val gt (val_abstract_ptr l π) (val_abstract_ptr l π')
-  | tr_val_array : forall gt a a',
+  | tr_val_array : forall a a',
       length a = length a' ->
       (forall i, 
-        index a i -> 
-        index a' i /\ tr_val gt a[i] a'[i]) ->
+        index a i -> tr_val gt a[i] a'[i]) -> 
       tr_val gt (val_array a) (val_array a')
-  | tr_val_struct : forall gt s s',
+  | tr_val_struct : forall s s',
       dom s = dom s' ->
       (forall f,
         index s f ->
@@ -73,8 +73,8 @@ Inductive tr_val : group_tr -> val -> val -> Prop :=
       tr_val gt (val_struct s) (val_struct s').
 
 (* S ~ |S| *)
-Inductive tr_stack : group_tr -> stack -> stack -> Prop :=
-  | tr_stack_intro : forall gt S S',
+Inductive tr_stack (gt:group_tr) : stack -> stack -> Prop :=
+  | tr_stack_intro : forall S S',
       List.map fst S = List.map fst S' ->
       (forall x v v',
         Ctx.lookup x S = Some v ->
@@ -82,8 +82,8 @@ Inductive tr_stack : group_tr -> stack -> stack -> Prop :=
       tr_stack gt S S'.
 
 (* m ~ |m| *)
-Inductive tr_state : group_tr -> state -> state -> Prop :=
-  | tr_state_intro : forall gt m m',
+Inductive tr_state (gt:group_tr) : state -> state -> Prop :=
+  | tr_state_intro : forall m m',
       dom m = dom m' ->
       (forall l,
         index m l ->
@@ -91,53 +91,93 @@ Inductive tr_state : group_tr -> state -> state -> Prop :=
       tr_state gt m m'.
 
 (* t ~ |t| *)
-Inductive tr_trm : trm -> trm -> Prop :=
+Inductive tr_trm (gt:group_tr) : trm -> trm -> Prop :=
   | tr_trm_val : forall v v',
-      tr_val v v' ->
-      tr_trm (trm_val v) (trm_val v')
+      tr_val gt v v' ->
+      tr_trm gt (trm_val v) (trm_val v')
   | tr_trm_var : forall x,
-      tr_trm (trm_var x) (trm_var x)
+      tr_trm gt (trm_var x) (trm_var x)
   | tr_trm_if : forall t1 t2 t3 t1' t2' t3',
-      tr_trm t1 t1' ->
-      tr_trm t2 t2' ->
-      tr_trm t3 t3' ->
-      tr_trm (trm_if t1 t2 t3) (trm_if t1' t2' t3')
+      tr_trm gt t1 t1' ->
+      tr_trm gt t2 t2' ->
+      tr_trm gt t3 t3' ->
+      tr_trm gt (trm_if t1 t2 t3) (trm_if t1' t2' t3')
   | tr_trm_let : forall x t1 t2 t1' t2',
-      tr_trm t1 t1' ->
-      tr_trm t2 t2' ->
-      tr_trm (trm_let x t1 t2) (trm_let x t1' t2')
+      tr_trm gt t1 t1' ->
+      tr_trm gt t2 t2' ->
+      tr_trm gt (trm_let x t1 t2) (trm_let x t1' t2')
   | tr_trm_binop : forall t1 t2 t1' t2',
-      tr_trm t1 t1' ->
-      tr_trm t2 t2' ->
-      tr_trm (trm_app binop_add (t1::t2::nil)) (trm_app binop_add (t1'::t2'::nil))
+      tr_trm gt t1 t1' ->
+      tr_trm gt t2 t2' ->
+      tr_trm gt (trm_app binop_add (t1::t2::nil)) (trm_app binop_add (t1'::t2'::nil))
   (* Abstract heap operations *)
   | tr_trm_get : forall T p p',
-      tr_trm p p' ->
-      tr_trm (trm_app (prim_get T) (p::nil)) (trm_app (prim_get T) (p'::nil))
+      tr_trm gt p p' ->
+      tr_trm gt (trm_app (prim_get T) (p::nil)) (trm_app (prim_get T) (p'::nil))
   | tr_trm_set : forall T p p' t t',
-      tr_trm p p' ->
-      tr_trm t t' ->
-      tr_trm (trm_app (prim_set T) (p::t::nil)) (trm_app (prim_set T) (p'::t'::nil))
+      tr_trm gt p p' ->
+      tr_trm gt t t' ->
+      tr_trm gt (trm_app (prim_set T) (p::t::nil)) (trm_app (prim_set T) (p'::t'::nil))
   | tr_trm_new : forall T t t',
-      tr_trm t t' ->
-      tr_trm (trm_app (prim_new T) (t::nil)) (trm_app (prim_new T) (t'::nil))
+      tr_trm gt t t' ->
+      tr_trm gt (trm_app (prim_new T) (t::nil)) (trm_app (prim_new T) (t'::nil))
   | tr_trm_array_access : forall A t i t' i' r,
-      tr_trm t t' ->
-      tr_trm i i' ->
+      tr_trm gt t t' ->
+      tr_trm gt i i' ->
       r = trm_app (prim_array_access A) (t'::i'::nil) ->
-      tr_trm (trm_app (prim_array_access A) (t::i::nil)) r
+      tr_trm gt (trm_app (prim_array_access A) (t::i::nil)) r
   (* Special case: struct access *)
-  | tr_trm_struct_access_x : forall p p' a1 a2 r,
-      tr_trm p p' ->
-      a1 = prim_struct_access (typ_struct "struct_x") "x" ->
-      a2 = prim_struct_access (typ_struct "pos") "s" ->
+  | tr_trm_struct_access_x : forall p p' s s_g f f_g a1 a2 r,
+      tr_trm gt p p' ->
+      s = group_tr_struct_name gt ->
+      s_g = group_tr_new_struct_name gt ->
+      mem f (group_tr_fields gt) ->
+      f_g = group_tr_new_struct_field gt ->
+      a1 = prim_struct_access (typ_struct s_g) f ->
+      a2 = prim_struct_access (typ_struct s) f_g ->
       r = trm_app a1 ((trm_app a2 (p'::nil))::nil) ->
-      tr_trm (trm_app (prim_struct_access (typ_struct "pos") "x") (p::nil)) r
-  | tr_trm_struct_access_other : forall p p' T f r,
-      (T <> "pos" \/ f <> "x") -> 
-      tr_trm p p' -> 
+      tr_trm gt (trm_app (prim_struct_access (typ_struct s) f) (p::nil)) r
+  | tr_trm_struct_access_other : forall s p p' T f r,
+      s = group_tr_struct_name gt ->
+      (T <> s \/ ~ mem f (group_tr_fields gt)) -> 
+      tr_trm gt p p' -> 
       r = (trm_app (prim_struct_access (typ_struct T) f) (p'::nil)) ->
-      tr_trm (trm_app (prim_struct_access (typ_struct T) f) (p::nil)) r.
+      tr_trm gt (trm_app (prim_struct_access (typ_struct T) f) (p::nil)) r.
+
+Lemma index_of_index_length' : forall A (l' l : list A) i,
+  index l' i ->
+  length l' = length l ->
+  index l i.
+Proof.
+  intros. rewrite index_eq_index_length in *.
+  applys* index_of_index_length'.
+Qed.
+
+Hint Resolve index_of_index_length'.
+
+(* Transformations are functions. *)
+Theorem functional_tr_accesses : forall gt π π1 π2,
+  tr_accesses gt π π1 ->
+  tr_accesses gt π π2 ->
+    π1 = π2.
+Proof.
+  induction π, π1, π2; introv H1 H2; inverts* H1 as; inverts* H2 as.
+  { introv H1 H2. forwards* Heq: IHπ H1 H2. rewrite* Heq. }
+  { introv H1 _ H2 _. forwards* Heq: IHπ H1 H2. rewrite* Heq. }
+  { introv H1 _ H2 _. forwards* Heq: IHπ H1 H2. rewrite* Heq. }
+Qed.
+
+Theorem functional_tr_val : forall gt v v1 v2,
+  tr_val gt v v1 ->
+  tr_val gt v v2 ->
+  v1 = v2.
+Proof.
+  introv H1 H2. gen v2. induction H1; intros; inverts H2; fequals.
+  { applys* functional_tr_accesses. }
+  { applys* eq_of_extens. math. }
+  { admit. }
+Qed.
+ 
 
 (* Semantics preserved by tr. *)
 Theorem red_tr: forall t t' v v' S S' m1 m1' m2 m2',
